Test/dafny0/ParallelResolveErrors.dfy
@@ -85,3 +85,67 @@ method M1() {
     }
   }
 }
+
+// -------------------------------------------------------------------------------------
+// Some soundness considerations
+// -------------------------------------------------------------------------------------
+
+ghost static method X_M0(y: int)
+  ensures exists o: object :: o != null && fresh(o);  // error: not allowed 'fresh' here
+{
+  var p := new object;
+}
+
+class X_C { ghost var data: int; }
+ghost static method X_M1(y: int)
+  ensures exists c: X_C :: c != null && c.data != old(c.data);  // error: not allowed 'old' here
+{
+  var c := new X_C;
+  c.data := c.data + 1;
+}
+
+method X_Main() {
+  if (*) {
+    parallel (x) { X_M0(x); }
+  } else {
+    parallel (x) { X_M1(x); }
+  }
+  assert false;
+}
+
+
+// The following seems to be a legitimate use of a two-state predicate in the postcondition of the parallel statement
+method X_Legit(c: X_C)
+  requires c != null;
+  modifies c;
+{
+  c.data := c.data + 1;
+  parallel (x | c.data <= x)
+    ensures old(c.data) < x;  // error: not allowed 'old' here
+  {
+  }
+}
+
+// X_M2 is like X_M0, but with an out-parameter
+ghost static method X_M2(y: int) returns (r: int)
+  ensures exists o: object :: o != null && fresh(o);  // 'fresh' is allowed here (because there's something coming "out" of this ghost method, namely 'r'
+{
+  var p := new object;
+}
+
+// The following method exhibits a case where M2 and a two-state parallel ensures would lead to an unsoundness
+// with the current translation.
+method X_AnotherMain(c: X_C)
+  requires c != null;
+  modifies c;
+{
+  c.data := c.data + 1;
+  parallel (x: int)
+    ensures exists o: object :: o != null && fresh(o);  // error: not allowed 'fresh' here
+  {
+    var s := X_M2(x);
+  }
+  assert false;
+}
+
+// -------------------------------------------------------------------------------------
